Add the fine-grained bag implementation

theories/hocap/cg_bag.v
@@ -61,44 +61,44 @@ Section proof.
 
   Definition bag_inv (γb : gname) (b : loc) : iProp Σ :=
     (∃ ls : list val, b ↦ (val_of_list ls) ∗ own γb ((1/2)%Qp, to_agree (of_list ls)))%I.
-  Definition isBag (γb : gname) (x : val) :=
+  Definition is_bag (γb : gname) (x : val) :=
 
     (∃ (lk : val) (b : loc) (γ : gname),
         ⌜x = PairV #b lk⌝ ∗ is_lock N γ lk (bag_inv γb b))%I.
-  Definition bagContents (γb : gname) (X : gmultiset val) : iProp Σ :=
+  Definition bag_contents (γb : gname) (X : gmultiset val) : iProp Σ :=
     own γb ((1/2)%Qp, to_agree X).
 
-  Global Instance isBag_persistent γb x : Persistent (isBag γb x).
+  Global Instance is_bag_persistent γb x : Persistent (is_bag γb x).
   Proof. apply _. Qed.
-  Global Instance bagContents_timeless γb X : Timeless (bagContents γb X).
+  Global Instance bag_contents_timeless γb X : Timeless (bag_contents γb X).
   Proof. apply _. Qed.
 
-  Lemma bagContents_agree γb X Y :
-    bagContents γb X -∗ bagContents γb Y -∗ ⌜X = Y⌝.
+  Lemma bag_contents_agree γb X Y :
+    bag_contents γb X -∗ bag_contents γb Y -∗ ⌜X = Y⌝.
   Proof.
-    rewrite /bagContents. apply uPred.wand_intro_r.
+    rewrite /bag_contents. apply uPred.wand_intro_r.
     rewrite -own_op own_valid uPred.discrete_valid.
     f_equiv=> /=. rewrite pair_op.
     by intros [_ ?%agree_op_invL'].
   Qed.
 
-  Lemma bagContents_update γb X X' Y :
-    bagContents γb X ∗ bagContents γb X' ==∗ bagContents γb Y ∗ bagContents γb Y.
+  Lemma bag_contents_update γb X X' Y :
+    bag_contents γb X ∗ bag_contents γb X' ==∗ bag_contents γb Y ∗ bag_contents γb Y.
   Proof.
     iIntros "[Hb1 Hb2]".
-    iDestruct (bagContents_agree with "Hb1 Hb2") as %<-.
+    iDestruct (bag_contents_agree with "Hb1 Hb2") as %<-.
     iMod (own_update_2 with "Hb1 Hb2") as "Hb".
     { rewrite pair_op frac_op'.
       assert ((1 / 2 + 1 / 2)%Qp = 1%Qp) as -> by apply Qp_div_2.
       by apply (cmra_update_exclusive (1%Qp, to_agree Y)). }
     iDestruct "Hb" as "[Hb1 Hb2]".
-    rewrite /bagContents. by iFrame.
+    rewrite /bag_contents. by iFrame.
   Qed.
 
   Lemma newBag_spec :
     {{{ True }}}
       newBag #()
-    {{{ x γ, RET x; isBag γ x ∗ bagContents γ ∅ }}}.
+    {{{ x γ, RET x; is_bag γ x ∗ bag_contents γ ∅ }}}.
   Proof.
     iIntros (Φ) "_ HΦ".
     unfold newBag. wp_rec.
@@ -108,30 +108,31 @@ Section proof.
     { iExists []. iFrame. }
     iIntros (lk γ) "#Hlk".
     iApply wp_value. iApply "HΦ".
-    rewrite /isBag /bagContents. iFrame.
+    rewrite /is_bag /bag_contents. iFrame.
     iExists _,_,_. by iFrame "Hlk".
   Qed.
 
   Local Opaque acquire release. (* so that wp_pure doesn't stumble *)
   Lemma pushBag_spec (P Q : iProp Σ) γ (x v : val)  :
-    □ (∀ (X : gmultiset val), bagContents γ X ∗ P
-                     ={⊤}=∗ ▷ (bagContents γ ({[v]} ∪ X) ∗ Q)) -∗
-    {{{ isBag γ x ∗ P }}}
+    □ (∀ (X : gmultiset val), bag_contents γ X ∗ P
+                     ={⊤∖↑N}=∗ ▷ (bag_contents γ ({[v]} ∪ X) ∗ Q)) -∗
+    {{{ is_bag γ x ∗ P }}}
       pushBag x (of_val v)
     {{{ RET #(); Q }}}.
   Proof.
     iIntros "#Hvs".
     iIntros (Φ). iAlways. iIntros "[#Hbag HP] HΦ".
     unfold pushBag. do 2 wp_rec.
-    rewrite /isBag /bag_inv.
+    rewrite /is_bag /bag_inv.
     iDestruct "Hbag" as (lk b γl) "[% #Hlk]"; simplify_eq/=.
     repeat wp_pure _.
     wp_apply (acquire_spec with "Hlk"). iIntros "[Htok Hb1]".
     iDestruct "Hb1" as (ls) "[Hb Ha]".
     wp_seq. wp_load. wp_let.
-    (* iApply (wp_mask_mono _ (⊤∖↑N)); first done. *)
+    wp_bind (_ <- _)%E.
+    iApply (wp_mask_mono _ (⊤∖↑N)); first done.
     iMod ("Hvs" with "[$Ha $HP]") as "[Hbc HQ]".
-    wp_store.
+    wp_store. wp_let.
     wp_apply (release_spec with  "[$Hlk $Htok Hbc Hb]").
     { iExists (v::ls); iFrame. }
     iIntros "_". by iApply "HΦ".
@@ -139,29 +140,31 @@ Section proof.
 
   Lemma popBag_spec (P : iProp Σ) (Q : val → iProp Σ) γ x :
     □ (∀ (X : gmultiset val) (y : val),
-               bagContents γ ({[y]} ∪ X) ∗ P
-               ={⊤}=∗ ▷ (bagContents γ X ∗ Q (SOMEV y))) -∗
-    □ (bagContents γ ∅ ∗ P ={⊤}=∗ ▷ (bagContents γ ∅ ∗ Q NONEV)) -∗
-    {{{ isBag γ x ∗ P }}}
+               bag_contents γ ({[y]} ∪ X) ∗ P
+               ={⊤∖↑N}=∗ ▷ (bag_contents γ X ∗ Q (SOMEV y))) -∗
+    □ (bag_contents γ ∅ ∗ P ={⊤∖↑N}=∗ ▷ (bag_contents γ ∅ ∗ Q NONEV)) -∗
+    {{{ is_bag γ x ∗ P }}}
       popBag x
     {{{ v, RET v; Q v }}}.
   Proof.
     iIntros "#Hvs1 #Hvs2".
     iIntros (Φ). iAlways. iIntros "[#Hbag HP] HΦ".
     unfold popBag. wp_rec.
-    rewrite /isBag /bag_inv.
+    rewrite /is_bag /bag_inv.
     iDestruct "Hbag" as (lk b γl) "[% #Hlk]"; simplify_eq/=.
     repeat wp_pure _.
     wp_apply (acquire_spec with "Hlk"). iIntros "[Htok Hb1]".
     iDestruct "Hb1" as (ls) "[Hb Ha]".
-    wp_seq. wp_load. destruct ls as [|v ls]; simpl.
+    wp_seq. wp_bind (!#b)%E.
+    iApply (wp_mask_mono _ (⊤∖↑N)); first done.
+    destruct ls as [|v ls]; simpl.
     - iMod ("Hvs2" with "[$Ha $HP]") as "[Hbc HQ]".
-      repeat wp_pure _.
+      wp_load. repeat wp_pure _.
       wp_apply (release_spec with  "[$Hlk $Htok Hbc Hb]").
       { iExists []; iFrame. }
       iIntros "_". repeat wp_pure _. by iApply "HΦ".
     - iMod ("Hvs1" with "[$Ha $HP]") as "[Hbc HQ]".
-      repeat wp_pure _. wp_store. do 2 wp_pure _.
+      wp_load. repeat wp_pure _. wp_store. do 2 wp_pure _.
       wp_apply (release_spec with  "[$Hlk $Htok Hbc Hb]").
       { iExists ls; iFrame. }
       iIntros "_". repeat wp_pure _. by iApply "HΦ".
@@ -169,14 +172,14 @@ Section proof.
 
 End proof.
 
-Typeclasses Opaque bagContents isBag.
+Typeclasses Opaque bag_contents is_bag.
 
 Canonical Structure cg_bag `{!heapG Σ, !bagG Σ} : bag Σ :=
-  {| is_bag := isBag;
-     is_bag_persistent := isBag_persistent;
-     bag_contents_timeless := bagContents_timeless;
-     bag_contents_agree := bagContents_agree;
-     bag_contents_update := bagContents_update;
+  {| abstract_bag.is_bag := is_bag;
+     abstract_bag.is_bag_persistent := is_bag_persistent;
+     abstract_bag.bag_contents_timeless := bag_contents_timeless;
+     abstract_bag.bag_contents_agree := bag_contents_agree;
+     abstract_bag.bag_contents_update := bag_contents_update;
      abstract_bag.newBag_spec := newBag_spec;
      abstract_bag.pushBag_spec := pushBag_spec;
      abstract_bag.popBag_spec := popBag_spec |}.
